Implement and verify a function: md5_of (file or stdin)

examples/md5ProgScript.sml
@@ -1,18 +1,18 @@
 (*
   Translate md5 function
 *)
-open preamble basis md5Theory;
+open preamble basis md5Theory UnsafeProgTheory cfLib basisFunctionsLib;
 
 val _ = new_theory "md5Prog"
 
-val _ = translation_extends "basisProg";
+val _ = translation_extends "UnsafeProg";
 
 (* translate md5Theory *)
 
 val res = translate w64_zero_def;
 val res = translate packLittle_def;
 val res = translate PADDING_def;
-val res = translate init_def;
+val init_v = translate init_def;
 val res = translate DROP_def;
 val res = translate subVec_def;
 
@@ -49,7 +49,7 @@ val res = translate (update1_def |> REWRITE_RULE [mul8add_simp]);
 val res = translate mul8add_thm;
 val res = translate genlist_rev_def;
 val res = translate update_def;
-val res = translate final_def;
+val final_v = translate final_def;
 val res = translate hxd_def;
 val res = translate EL;
 
@@ -76,6 +76,90 @@ QED
 val _ = update_precondition byte2hex_side_thm;
 
 val res = translate toHexString_def;
-val res = translate (md5_def |> SIMP_RULE std_ss [o_DEF]);
+
+Definition md5_update_def:
+  md5_update y x = update1 x (n2w (ORD y))
+End
+
+val md5_update_v = translate md5_update_def;
+
+Definition md5_final_def:
+  md5_final s = SOME (implode (toHexString (final s)))
+End
+
+val md5_final_v = translate md5_final_def;
+
+val md5_lem = md5_def
+  |> SIMP_RULE std_ss [FOLDL_MAP,mllistTheory.foldl_intro,GSYM md5_update_def]
+  |> CONV_RULE (DEPTH_CONV ETA_CONV);
+
+val res = translate md5_lem;
+
+val _ = (append_prog o process_topdecs) `
+  fun md5_of stdin_or_fname =
+    case TextIO.foldChars md5_update init stdin_or_fname of
+      Some s => md5_final s
+    | None => None`;
+
+Theorem md5_of_v_def = fetch "-" "md5_of_v_def";
+
+Theorem md5_of_SOME:
+  OPTION_TYPE FILENAME (SOME s) fnv ∧
+  hasFreeFD fs
+  ⇒
+  app (p:'ffi ffi_proj) md5_of_v [fnv]
+    (STDIO fs)
+    (POSTv retv. STDIO fs *
+                 & (OPTION_TYPE STRING_TYPE
+                      (OPTION_MAP (implode o md5) (file_content fs s))
+                      retv))
+Proof
+  rpt strip_tac
+  \\ xcf_with_def "md5_of" md5_of_v_def
+  \\ assume_tac md5_update_v
+  \\ assume_tac init_v
+  \\ drule_all (foldChars_SOME |> GEN_ALL)
+  \\ disch_then (assume_tac o SPEC_ALL)
+  \\ xlet ‘(POSTv retv.
+             STDIO fs *
+             &OPTION_TYPE MD5_MD5STATE_TYPE
+               (OPTION_MAP (foldl md5_update init) (file_content fs s)) retv)’
+  THEN1 xapp
+  \\ Cases_on ‘file_content fs s’ \\ fs []
+  \\ gvs [std_preludeTheory.OPTION_TYPE_def]
+  \\ xmatch THEN1 (xcon \\ xsimpl)
+  \\ xapp \\ xsimpl
+  \\ first_x_assum $ irule_at (Pos hd) \\ rw []
+  \\ gvs [std_preludeTheory.OPTION_TYPE_def,md5_final_def]
+  \\ fs [md5_lem]
+QED
+
+Theorem md5_of_NONE:
+  OPTION_TYPE FILENAME NONE fnv ∧
+  stdin_content fs = SOME text
+  ⇒
+  app (p:'ffi ffi_proj) md5_of_v [fnv]
+    (STDIO fs)
+    (POSTv retv. STDIO (fastForwardFD fs 0) *
+                 & (OPTION_TYPE STRING_TYPE (SOME (implode (md5 text))) retv))
+Proof
+  rpt strip_tac
+  \\ xcf_with_def "md5_of" md5_of_v_def
+  \\ assume_tac md5_update_v
+  \\ assume_tac init_v
+  \\ drule_all (foldChars_NONE |> GEN_ALL)
+  \\ disch_then (assume_tac o SPEC_ALL)
+  \\ xlet ‘(POSTv retv.
+             STDIO (fastForwardFD fs 0) *
+             &OPTION_TYPE MD5_MD5STATE_TYPE
+               (SOME (foldl md5_update init text)) retv)’
+  THEN1 xapp
+  \\ gvs [std_preludeTheory.OPTION_TYPE_def]
+  \\ xmatch
+  \\ xapp \\ xsimpl
+  \\ first_x_assum $ irule_at (Pos hd) \\ rw []
+  \\ gvs [std_preludeTheory.OPTION_TYPE_def,md5_final_def]
+  \\ fs [md5_lem]
+QED
 
 val _ = export_theory();
